WIP on specification"

src/specification.lean
@@ -1,42 +1,99 @@
 -- trying to formulize ideas from Efficient Building Blocks for Delay Insensitive Circuits
 -- by Priyanarsan Patra and Donald S. Fussell - University of Texas at Austin
-import data.finset
-import data.multiset.nodup
 
-namespace specification
+-- namespace specification
+
+import data.list
+
+inductive set.star {α : Type} : set (list α) → (list α) → Prop
+  | nil : ∀ {s}, set.star s list.nil
+  | here : ∀ s l rest, l ∈ s → set.star s rest → set.star s (l ++ rest)
+
+inductive shuffle {α : Type} : list α → list α → list α → Prop
+  | nil : shuffle [] [] []
+  | from_left : ∀ {l l_left l_right} (x : α), 
+    shuffle l l_left l_right → shuffle (x::l) l_left (x::l_right)
+  | from_right : ∀ {l l_left l_right} (x : α),
+    shuffle l l_left l_right → shuffle (x::l) (x::l_left) l_right
 
 structure event :=
   (is_output : bool) (name : string)
 
-postfix ! := λ s, {event . is_output := true, name := s }
-postfix ? := λ s, {event . is_output := false, name := s }
+postfix `!` := λ s, {event . is_output := true, name := s }
+postfix `?` := λ s, {event . is_output := false, name := s }
 
-def behavior := finset (list event)
+class trace_structure (α : Type) extends has_mem (list event) α, has_emptyc α :=
+  (pref : α → α)
+  (and_then : α → α → α)
+  (par : α → α → α)
+  (nondet : α → α → α)
+  (star : α → α)
 
-lemma list.inits.nodup {α} (l : list α) : l.inits.nodup :=
-  by {
-    induction l, 
-    
-    case nil {
-      apply list.nodup_cons.mpr,
-      simp only [list.not_mem_nil, not_false_iff, and_self, list.nodup_nil],
+abbreviation pref {α} [trace_structure α] (a : α) := trace_structure.pref a 
+infix `⬝` := λ {α} [trace_structure α] (a b : α), trace_structure.and_then a b
+infix `∥`:60 := λ {α} [trace_structure α] (a b : α), trace_structure.par a b
+infix `|`:60 := λ {α} [trace_structure α] (a b : α), trace_structure.nondet a b
+prefix `⋆`:60 := λ {α} [trace_structure α] (a : α), (trace_structure.star a : α) 
+
+class lawful_trace_structure (α : Type) extends trace_structure α :=
+  (pref_idempotent : ∀ a : α, pref (pref a) = pref a)
+  (star_idempotent : ∀ a : α, ⋆(⋆a) = ⋆a)
+  (and_then_assoc : ∀ a b c : α, a⬝b⬝c = a⬝(b⬝c))
+  (par_assoc : ∀ a b c : α, a∥b∥c = a∥(b∥c))
+  (nondet_assoc : ∀ a b c : α, a|b|c = a|(b|c))
+  (star_unfold : ∀ a : α, ⋆a = (∅|(a⬝(⋆a) : α)))
+
+def on_sets {α} (op : α → α → α → Prop) (s₀ s₁ : set α) : set α :=
+  λ a, ∃ a₀ a₁, a₀ ∈ s₀ ∧ a₁ ∈ s₁ ∧ op a a₀ a₁
+
+instance : trace_structure (set (list event) : Type) :=
+{ 
+  pref := λ s l, exists l', l' ∈ s ∧ l <+: l,
+  and_then := on_sets (λ l l₀ l₁, l = l₀ ++ l₁),
+  par := on_sets shuffle,
+  nondet := set.union,
+  star := set.star,
+  .. set.has_mem,
+  .. set.has_emptyc
+}
+
+instance : lawful_trace_structure (set (list event)) :=
+{ 
+  pref_idempotent := by {
+    intros s,
+    unfold_projs,
+    ext; split; intros h; rcases h with ⟨y, y_mem, h⟩,
+    {
+      simp only [exists_and_distrib_right] at y_mem,
+      unfold set.mem at y_mem,
+      rcases y_mem with ⟨⟨z, z_in_s⟩, y_prefix⟩,
+      use z,
+      split, 
+      {exact (set.mem.equations._eqn_1 z s).mpr z_in_s},
+      {exact h},
     },
-
-    case cons {
-      simp only [true_and, list.inits, list.mem_map, exists_false, not_false_iff, list.nodup_cons, and_false],
-      apply list.nodup_map list.cons_injective l_ih,
+    {
+      use y,
+      split,
+      apply (set.mem.equations._eqn_1 _ _).mpr,
+      simp only [exists_and_distrib_right],
+      use y, exact y_mem, exact h
     }
-  }
-
-def prefix_close {α} [decidable_eq α] (s : finset (list α)) : finset (list α) :=
-  s.bUnion (λ l, ⟨l.inits, list.inits.nodup l⟩)
-
-def and_then {α} [decidable_eq α] (s₀ s₁ : finset (list α)) : finset (list α) :=
-  s₀.bUnion (λ l₀, s₁.map (⟨(λ l₁, l₀ ++ l₁), by {refine list.append_right_injective l₀}⟩ )
-
-def shuffle {α} [decidable_eq α] : list α → list α → finset (list α)
-  | [] l₁ := {l₁}
-  | l₀ [] := {l₀}
-  | (x₀::xs₀) (x₁::xs₁) := (shuffle xs₀ (x₁ :: xs₁)).map ⟨λ l, 
+  },
+  star_idempotent := by {
+    intros s,
+    unfold trace_structure.star,
+    ext; split; intros h; cases h with _ _ l h_rest l_in_star star_star,
+    {apply set.star.nil},
+    {
+      cases l_in_star,
+    }
+  },
+  and_then_assoc := _,
+  par_assoc := _,
+  nondet_assoc := _,
+  star_unfold := _,
+  .. set.trace_structure
+}
 
 end specification
